vale/code/crypto/aes/GHash.fsti
@@ -49,6 +49,7 @@ let hkeys_reqs_priv (hkeys:seq quad32) (h_BE:quad32) : Prop_s.prop0
   of_quad32 (index hkeys 1) == gf128_power h 2 /\
   of_quad32 (index hkeys 3) == gf128_power h 3 /\
   of_quad32 (index hkeys 4) == gf128_power h 4 /\
+  index hkeys 5 = Mkfour 0 0 0 0 /\
   of_quad32 (index hkeys 6) == gf128_power h 5 /\
   of_quad32 (index hkeys 7) == gf128_power h 6 
 
