vale/code/crypto/aes/OptPublic.fsti
@@ -2,6 +2,12 @@ module OptPublic
 
 open Types_s
 
-val hkeys_reqs_pub (hkeys:FStar.Seq.seq quad32) (h_LE:quad32) : Prop_s.prop0
+val hkeys_reqs_pub (hkeys:FStar.Seq.seq quad32) (h_BE:quad32) : Prop_s.prop0
 
-val get_hkeys_reqs (h_LE:quad32) : (s:Seq.lseq quad32 8{hkeys_reqs_pub s h_LE})
+val get_hkeys_reqs (h_BE:quad32) : (s:Seq.lseq quad32 8{hkeys_reqs_pub s h_BE})
+
+val get_hkeys_reqs_injective (h_BE:quad32) (s1 s2:Seq.seq quad32) : Lemma
+  (requires 
+    Seq.length s1 = 8 /\ Seq.length s2 = 8 /\
+    hkeys_reqs_pub s1 h_BE /\ hkeys_reqs_pub s2 h_BE)
+  (ensures s1 == s2)
